Spec/Assert.lean
@@ -1,0 +1,9 @@
+module
+public import Spec.Assert.Assert
+public import Spec.Assert.Base
+public import Spec.Assert.HashMap
+public import Spec.Assert.IO
+public import Spec.Assert.Ordering
+public import Spec.Assert.Pred
+public import Spec.Assert.TempDir
+public import Spec.Assert.String
