Spec/Assert/Base.lean
@@ -1,0 +1,20 @@
+module
+public import Init.System.IO
+public import Lean.Data.RBTree
+public import Lean
+public import Lean.Data.RBMap
+public import Std.Data.HashSet
+public import Lean.Data.RBTree
+public import Init.System.IO
+public import Lean.Elab.Term
+public import Lean.Parser.Term
+public import Init.Data.Repr
+
+@[expose] public section
+
+namespace Spec.Assert
+
+def fail (msg : String) : IO Unit := throw <| IO.Error.userError msg
+
+end Spec.Assert
+end
