Spec/Assert/Pred.lean
@@ -1,0 +1,17 @@
+module
+public import Spec.Assert.Base
+
+@[expose] public section
+
+namespace Spec.Assert
+
+def shouldSatisfy [ToString α] (actual : α) (pred : α → Bool) : IO Unit := do
+  unless pred actual do
+    fail s!"❌ {toString actual} doesn't satisfy predicate"
+
+def shouldNotSatisfy [ToString α] (actual : α) (pred : α → Bool) : IO Unit := do
+  if pred actual then
+    fail s!"❌ {toString actual} satisfies predicate, but should not"
+
+end Spec.Assert
+end
