Spec/Reporter.lean
@@ -1,0 +1,7 @@
+module
+public import Spec.Reporter.Base
+public import Spec.Reporter.Console
+public import Spec.Reporter.Dot
+public import Spec.Reporter.Spec
+public import Spec.Reporter.Tap
+public import Spec.Reporter.TeamCity
