Spec/Speed.lean
@@ -1,13 +1,14 @@
-import Spec.Style
-import Std.Time
+module
+public import Std.Time.Time.Unit.Millisecond
+
+@[expose] public section
 
 namespace Spec
 
-
 inductive Speed where
-  | fast -- fast__below_or_eq_half_threshold
-  | medium -- medium__more_half__and__less_or_eq_threshold
-  | slow -- slow_above_threshold
+  | fast
+  | medium
+  | slow
   deriving Repr, DecidableEq, Ord, Hashable
 
 namespace Speed
@@ -26,12 +27,7 @@ protected def speedOf_Millisecond (threshold ms : Std.Time.Millisecond.Offset) :
 protected def speedOf_Nat (threshold ms : Nat) : Speed :=
   Speed.speedOf_Int threshold ms
 
-protected def toStyle : Speed → List StyleModifier
-  | .fast   => Style.dim
-  | .medium => Style.yellow
-  | .slow   => Style.red
-
-protected def toString : Speed -> String
+protected def toString : Speed → String
   | .fast => "Speed.fast"
   | .medium => "Speed.medium"
   | .slow => "Speed.slow"
@@ -40,8 +36,5 @@ end Speed
 
 instance : ToString Speed := ⟨Speed.toString⟩
 
--- #guard Speed.speedOf_Nat 1000 1001 = Speed.slow
--- #guard Speed.speedOf_Nat 1000 1000 = Speed.medium
--- #guard Speed.speedOf_Nat 1000 600 = Speed.medium
--- #guard Speed.speedOf_Nat 1000 501 = Speed.medium
--- #guard Speed.speedOf_Nat 1000 500 = Speed.fast
+end Spec
+end
