SpecExtraFileTree.lean
@@ -1,0 +1,4 @@
+module
+prelude
+public import SpecExtraFileTree.WithTree
+public import SpecExtraFileTree.Data.Tree
