SpecExtraFileTree/WithTree.lean
@@ -1,0 +1,32 @@
+module
+public import SpecExtraFileTree.Data.Tree
+public import Init.System.IO
+
+@[expose] public section
+
+open System in
+def Tree_createAtPath : Tree → FilePath → IO Unit
+  | Tree.file name, path => do
+    let fullPath := path / name
+    IO.FS.writeFile fullPath "" -- create empty file
+  | Tree.dir name children, path => do
+    let dirPath := path / name
+    IO.FS.createDirAll dirPath
+    for child in children do
+      Tree_createAtPath child dirPath
+
+def createAtPathForest (trees : List Tree) (path : FilePath) : IO Unit :=
+  for tree in trees do
+    Tree_createAtPath tree path
+
+def withTempDirTree (t : Tree) (cont : FilePath → IO α) : IO α :=
+  IO.FS.withTempDir fun tmpDir => do Tree_createAtPath t tmpDir; cont tmpDir
+
+def withTempDirForest (trees : List Tree) (cont : FilePath → IO α) : IO α :=
+  IO.FS.withTempDir fun tmpDir => do createAtPathForest trees tmpDir; cont tmpDir
+
+-- def withinTempDirTree (t : Tree) (cont : FilePath → IO α) : IO α :=
+--   withTempDirTree t (fun tmpDir => do IO.Process.setCurrentDir tmpDir; cont tmpDir)
+
+-- def withinTempDirForest (ts : List Tree) (cont : FilePath → IO α) : IO α :=
+--   withTempDirForest ts (fun tmpDir => do IO.Process.setCurrentDir tmpDir; cont tmpDir)
